unify hole unchanged definitions and fix proof to account

compiler/backend/proofs/bvi_tmcProofScript.sml
@@ -546,19 +546,11 @@ Definition hole_has_val_def:
     FLOOKUP refs hole_ptr = SOME (MutBlock tag left c right)
 End
 
-Definition hole_unchanged_def:
-  hole_unchanged f refs refs' ⇔
-    ∀hole_ptr hole_val.
-      hole_ptr ∉ FRANGE f ∧
-      FLOOKUP refs hole_ptr = SOME hole_val ⇒
-      FLOOKUP refs' hole_ptr = SOME hole_val
-End
-
-Definition hole_unchanged'_def:
-  hole_unchanged' f refs refs' hole_ptr ⇔
+Definition holes_unchanged_except_def:
+  holes_unchanged_except f refs refs' changed ⇔
     ∀ptr val.
       ptr ∉ FRANGE f ∧
-      (∀b. RefPtr b ptr ≠ hole_ptr) ∧
+      (∀b. RefPtr b ptr ∉ changed) ∧
       FLOOKUP refs ptr = SOME val ⇒
       FLOOKUP refs' ptr = SOME val
 End
@@ -568,20 +560,20 @@ Definition only_fresh_def:
   ∀n. n ∈ FRANGE f' ∧ ~(n ∈ FRANGE f) ⇒ ~(n ∈ FDOM refs_old)
 End
 
-Theorem hole_unchanged_refl:
-  ∀f refs. hole_unchanged f refs refs
+Theorem holes_unchanged_except_refl:
+  ∀f refs changed. holes_unchanged_except f refs refs changed
 Proof
-  rw [hole_unchanged_def]
+  rw [holes_unchanged_except_def]
 QED
 
-Theorem hole_unchanged_submap:
-  ∀f f' refs refs'.
-    hole_unchanged f refs refs' ∧
+Theorem holes_unchanged_except_submap:
+  ∀f f' refs refs' changed.
+    holes_unchanged_except f refs refs' changed ∧
     f ⊑ f' ⇒
-    hole_unchanged f' refs refs'
+    holes_unchanged_except f' refs refs' changed
 Proof
-  rw [hole_unchanged_def]
-  >> first_x_assum $ qspecl_then [‘hole_ptr’, ‘hole_val’] mp_tac
+  rw [holes_unchanged_except_def]
+  >> first_x_assum $ qspecl_then [‘ptr’, ‘val’] mp_tac
   >> strip_tac
   >> gvs []
   >> pop_assum irule
@@ -591,16 +583,16 @@ Proof
   >> gvs [SUBSET_DEF]
 QED
 
-Theorem hole_unchanged_trans:
-  ∀f f' refs refs' refs''.
-    hole_unchanged f refs refs' ∧
-    hole_unchanged f' refs' refs'' ∧
+Theorem holes_unchanged_except_trans:
+  ∀f f' refs refs' refs'' changed.
+    holes_unchanged_except f refs refs' changed ∧
+    holes_unchanged_except f' refs' refs'' changed ∧
     only_fresh f f' refs ∧
     f ⊑ f' ⇒
-    hole_unchanged f refs refs''
+    holes_unchanged_except f refs refs'' changed
 Proof
-  rw [hole_unchanged_def]
-  >> rpt $ first_x_assum $ qspecl_then [‘hole_ptr’, ‘hole_val’] mp_tac
+  rw [holes_unchanged_except_def]
+  >> rpt $ first_x_assum $ qspecl_then [‘ptr’, ‘val’] mp_tac
   >> rpt strip_tac
   >> gvs []
   >> first_x_assum irule
@@ -611,30 +603,18 @@ Proof
   >> gvs [FLOOKUP_DEF]
 QED
 
-(* TODO *)
-Theorem hole_unchanged'_trans:
-  ∀f f' refs refs' refs''.
-    hole_unchanged f refs refs' ∧
-    hole_unchanged f' refs' refs'' ∧
-    only_fresh f f' refs ∧
-    f ⊑ f' ⇒
-    hole_unchanged f refs refs''
-Proof
-  cheat
-QED
-
 Theorem unchanged_hole_has_val:
-  ∀f f' env env' hole_ptr hole_idx refs refs' c.
+  ∀f f' env env' hole_ptr hole_idx refs refs' c changed.
     hole_has_val f env (env' ++ [RefPtr F hole_ptr; Number hole_idx]) refs c ∧
     only_fresh f f' refs ∧
-    hole_unchanged f refs refs' ∧
+    holes_unchanged_except f refs refs' ∅ ∧
     env_rel T f env (env' ++ [RefPtr F hole_ptr; Number hole_idx]) ⇒
     hole_has_val f' env (env' ++ [RefPtr F hole_ptr; Number hole_idx]) refs' c
 Proof
   rw [hole_has_val_def]
   >> drule env_rel_length_opt
   >> strip_tac
-  >> gvs [EL_APPEND_EQN, hole_unchanged_def]
+  >> gvs [EL_APPEND_EQN, holes_unchanged_except_def]
   >> first_x_assum drule_all
   >> strip_tac
   >> gvs []
@@ -764,7 +744,7 @@ Theorem evaluate_rewrite_tmc:
        state_rel f' t t' ∧
        f SUBMAP f' ∧
        only_fresh f f' s'.refs ∧
-       hole_unchanged f s'.refs t'.refs ∧
+       holes_unchanged_except f s'.refs t'.refs ∅ ∧
        (opt ⇒
         (∀loc loc_opt arity exp_aux exp_opt.
            rewrite_aux loc loc_opt arity (HD xs) = SOME exp_aux ⇒
@@ -780,16 +760,16 @@ Theorem evaluate_rewrite_tmc:
              evaluate ([exp_opt], env2, s') = (rrr,t2) ∧
              opt_res_rel r' rrr ∧
              state_rel f' t t2 ∧
-             hole_unchanged' f s'.refs t2.refs (EL i env2) ∧
+             holes_unchanged_except f s'.refs t2.refs {EL i env2} ∧
              ∀res_v.
                 r' = Rval [res_v] ⇒
                 hole_has_val f env1 env2 t2.refs res_v))
 Proof
 
   recInduct bviSemTheory.evaluate_ind
-  >> rpt strip_tac (*
+  >> rpt strip_tac
   >~ [‘evaluate ([],_,_)’] >-
-   (gvs [evaluate_def] >> first_x_assum $ irule_at Any >> fs [only_fresh_def, hole_unchanged_def])
+   (gvs [evaluate_def] >> first_x_assum $ irule_at Any >> fs [only_fresh_def, holes_unchanged_except_def])
   >~ [‘evaluate (x::y::xs,_,_)’] >-
    (gvs [evaluate_def]
     (* First inductive hypothesis *)
@@ -835,7 +815,7 @@ Proof
         >> rpt $ goal_assum $ drule_at Any
         >> irule evaluate_refs_SUBSET
         >> goal_assum $ drule_at Any)
-      >> irule hole_unchanged_trans
+      >> irule holes_unchanged_except_trans
       >> rpt $ goal_assum $ drule_at Any)
     >> rename [‘state_rel f3 t t'’]
     >> qexists ‘f3’ >> fs []
@@ -846,7 +826,7 @@ Proof
       >> rpt $ goal_assum $ drule_at Any
       >> irule evaluate_refs_SUBSET
       >> goal_assum $ drule_at Any)
-    >> irule hole_unchanged_trans
+    >> irule holes_unchanged_except_trans
     >> rpt $ goal_assum $ drule_at Any)
   >~ [‘Var n’] >-
    (gvs [evaluate_def]
@@ -860,44 +840,41 @@ Proof
     >> conj_tac
     >- (irule only_fresh_refl)
     >> conj_tac
-    >-
-     (strip_tac
-      >> gvs []
-      >> conj_tac
-      >- (rpt gen_tac >> gvs [rewrite_aux_def])
-      >> rpt gen_tac
-      >> gvs [opt_res_rel_def]
-      >> gvs [rewrite_opt_def]
-      (* Lemma for evaluating Op (MemOp UpdateCons)? *)
-      >> gvs [evaluate_def]
-      >> drule env_rel_length_opt
-      >> gvs []
-      >> strip_tac
-      >> gvs [do_app_def]
-      >> gvs [do_app_aux_def]
-      >> drule env_rel_extras_opt
-      >> strip_tac
-      >> gvs []
-      >> gvs [case_eq_thms]
-      >> gvs [PULL_EXISTS]
-      >> gvs [bvlSemTheory.Unit_def, backend_commonTheory.tuple_tag_def]
-      >> gvs [hole_has_val_def, FLOOKUP_SIMP]
-      >> gvs [state_rel_def, state_ref_rel_def, FLOOKUP_SIMP]
-      >> rpt strip_tac
-      >-
-        (last_x_assum drule
-         >> strip_tac
-         >> goal_assum $ drule_at Any
-         >> goal_assum $ drule_at Any
-         >> IF_CASES_TAC
-         >> gvs [flookup_thm, FRANGE_DEF])
-      >> gvs [hole_unchanged'_def]
-      >> gvs [FLOOKUP_SIMP]
-      >> rw []
-      >> metis_tac [])
+    >- irule holes_unchanged_except_refl
     >> strip_tac
     >> gvs []
-    >> irule hole_unchanged_refl)
+    >> conj_tac
+    >- (rpt gen_tac >> gvs [rewrite_aux_def])
+    >> rpt gen_tac
+    >> gvs [opt_res_rel_def]
+    >> gvs [rewrite_opt_def]
+    (* Lemma for evaluating Op (MemOp UpdateCons)? *)
+    >> gvs [evaluate_def]
+    >> drule env_rel_length_opt
+    >> gvs []
+    >> strip_tac
+    >> gvs [do_app_def]
+    >> gvs [do_app_aux_def]
+    >> drule env_rel_extras_opt
+    >> strip_tac
+    >> gvs []
+    >> gvs [case_eq_thms]
+    >> gvs [PULL_EXISTS]
+    >> gvs [bvlSemTheory.Unit_def, backend_commonTheory.tuple_tag_def]
+    >> gvs [hole_has_val_def, FLOOKUP_SIMP]
+    >> gvs [state_rel_def, state_ref_rel_def, FLOOKUP_SIMP]
+    >> rpt strip_tac
+    >-
+     (last_x_assum drule
+      >> strip_tac
+      >> goal_assum $ drule_at Any
+      >> goal_assum $ drule_at Any
+      >> IF_CASES_TAC
+      >> gvs [flookup_thm, FRANGE_DEF])
+    >> gvs [holes_unchanged_except_def]
+    >> gvs [FLOOKUP_SIMP]
+    >> rw []
+    >> metis_tac [])
   >~ [‘If x1 x2 x3’] >-     
    (gvs [evaluate_def]
     >> gvs [CaseEq "prod", PULL_EXISTS]
@@ -962,6 +939,10 @@ Proof
             >> qexistsl [‘env2’, ‘Rval [Boolv T]’, ‘[x1]’]
             >> gvs [])
           >-
+           (irule holes_unchanged_except_trans
+            >> first_assum $ irule_at Any
+            >> gvs [])
+          >-
            (drule aux_strip_if_then
             >> strip_tac
             >-
@@ -973,9 +954,14 @@ Proof
           >> first_x_assum $ qspecl_then [‘loc’, ‘loc_opt’] mp_tac
           >> strip_tac
           >> gvs [rewrite_opt_def, evaluate_def]
+          >> drule_all env_rel_length_opt
+          >> strip_tac
+          >> gvs [EL_APPEND_EQN]
           >> conj_tac
           >-
-           (cheat)
+           (irule holes_unchanged_except_trans
+            >> first_assum $ irule_at Any
+            >> gvs [holes_unchanged_except_def])
           >> gen_tac
           >> strip_tac
           >> first_x_assum $ qspec_then ‘res_v’ mp_tac
@@ -1023,6 +1009,10 @@ Proof
           >> qexistsl [‘env2’, ‘Rval [Boolv F]’, ‘[x1]’]
           >> gvs [])
         >-
+         (irule holes_unchanged_except_trans
+          >> first_assum $ irule_at Any
+          >> gvs [])
+        >-
          (drule aux_strip_if_else
           >> strip_tac
           >-
@@ -1034,8 +1024,14 @@ Proof
         >> first_x_assum $ qspecl_then [‘loc’, ‘loc_opt’] mp_tac
         >> strip_tac
         >> gvs [rewrite_opt_def, evaluate_def]
+        >> drule_all env_rel_length_opt
+        >> strip_tac
+        >> gvs [EL_APPEND_EQN]
         >> conj_tac
-        >- cheat
+        >-
+         (irule holes_unchanged_except_trans
+          >> first_assum $ irule_at Any
+          >> gvs [holes_unchanged_except_def])
         >> gen_tac
         >> strip_tac
         >> first_x_assum $ qspec_then ‘res_v’ mp_tac
@@ -1058,8 +1054,7 @@ Proof
        (drule aux_strip_if_then
         >> strip_tac
         >> gvs [evaluate_def])
-      >> gvs [rewrite_opt_def, evaluate_def, opt_res_rel_def]
-      >> gvs [hole_unchanged_def, hole_unchanged'_def]) (* TODO lemma *)
+      >> gvs [rewrite_opt_def, evaluate_def, opt_res_rel_def, holes_unchanged_except_def])
     (* Non opt *)
     (* First inductive hypothesis *)
     >> first_x_assum $ qspec_then ‘F’ mp_tac
@@ -1099,8 +1094,9 @@ Proof
           >> rpt $ goal_assum $ drule_at Any
           >> irule evaluate_refs_SUBSET
           >> rpt $ goal_assum $ drule_at Any)
-        >> irule hole_unchanged_trans
-        >> rpt $ goal_assum $ drule_at Any)
+        >> irule holes_unchanged_except_trans
+        >> first_assum $ irule_at Any
+        >> gvs [])
       (* else inductive hypothesis *)
       >> Cases_on ‘v1 = Boolv F’
       >> gvs []
@@ -1121,11 +1117,12 @@ Proof
         >> rpt $ goal_assum $ drule_at Any
         >> irule evaluate_refs_SUBSET
         >> rpt $ goal_assum $ drule_at Any)
-      >> irule hole_unchanged_trans
-      >> rpt $ goal_assum $ drule_at Any)
+      >> irule holes_unchanged_except_trans
+      >> first_assum $ irule_at Any
+      >> gvs [])
     >> qexists ‘f''’
     >> gvs [])
-  >~ [‘Let xs x2’] >-
+  >~ [‘Let xs x2’] >-     
    (gvs [evaluate_def]
     >> gvs [CaseEq "prod", PULL_EXISTS]
     >> rename [‘evaluate (xs,env,s) = (rs,u)’]
@@ -1164,11 +1161,12 @@ Proof
           >> strip_tac                        
           >> qexists ‘c’
           >> irule unchanged_hole_has_val
-          >> drule_all hole_unchanged_submap
+          >> drule_all holes_unchanged_except_submap
           >> strip_tac
-          >> goal_assum $ drule_at $ Pos hd
+          >> goal_assum $ drule_at $ Pos $ el 2
+          >> goal_assum $ drule_at $ Pos $ el 2
           >> rw []
-          >- irule only_fresh_refl
+          >- irule only_fresh_refl                        
           >> drule_at Any hole_has_val_append
           >> disch_then $ qspecl_then [‘s'.refs’, ‘env2 ++ [RefPtr F hole_ptr; Number hole_idx]’, ‘env’, ‘c’] mp_tac
           >> impl_tac
@@ -1176,7 +1174,7 @@ Proof
            (irule unchanged_hole_has_val
             >> goal_assum $ drule_at $ Pos $ el 4
             >> gvs []
-            >> simp [hole_unchanged_def])
+            >> simp [holes_unchanged_except_def])
           >> strip_tac
           >> gvs [])
         >> strip_tac
@@ -1194,6 +1192,10 @@ Proof
           >> irule evaluate_refs_SUBSET
           >> rpt $ goal_assum $ drule_at Any)
         >-
+         (irule holes_unchanged_except_trans
+          >> first_assum $ irule_at Any
+          >> gvs [])
+        >-
          (drule aux_strip_let
           >> strip_tac
           >> last_x_assum drule
@@ -1203,8 +1205,19 @@ Proof
         >> strip_tac
         >> rev_drule evaluate_IMP_LENGTH
         >> gvs [rewrite_opt_def, evaluate_def]
-        >> rpt strip_tac
-        >- (cheat)
+        >> strip_tac
+        >> drule_all env_rel_length_opt
+        >> strip_tac
+        >> drule LIST_REL_LENGTH
+        >> strip_tac
+        >> gvs [EL_APPEND_EQN]
+        >> conj_tac
+        >-
+         (irule holes_unchanged_except_trans
+          >> first_x_assum $ irule_at Any
+          >> gvs [holes_unchanged_except_def])
+        >> strip_tac
+        >> strip_tac
         >> first_x_assum drule
         >> strip_tac
         >> irule hole_has_val_submap
@@ -1226,7 +1239,7 @@ Proof
           >> strip_tac
           >> gvs [evaluate_def])
       >> gvs [rewrite_opt_def, evaluate_def, opt_res_rel_def]
-      >> gvs [hole_unchanged_def, hole_unchanged'_def])
+      >> gvs [holes_unchanged_except_def])
     (* Non-opt *)
     (* First inductive hypothesis *)
     >> first_x_assum $ qspec_then ‘F’ mp_tac
@@ -1256,10 +1269,10 @@ Proof
         >> rpt $ goal_assum $ drule_at Any
         >> irule evaluate_refs_SUBSET
         >> rpt $ goal_assum $ drule_at Any)
-      >> irule hole_unchanged_trans
+      >> irule holes_unchanged_except_trans
       >> rpt $ goal_assum $ drule_at Any)
     >> goal_assum $ drule_at Any
-    >> gvs []) *)
+    >> gvs [])
   >~ [‘Raise x’] >-
    (gvs [evaluate_def]
     >> gvs [CaseEq "prod", PULL_EXISTS]
@@ -1278,8 +1291,7 @@ Proof
       >> Cases_on ‘v’
       >> gvs [rewrite_aux_def, rewrite_opt_def, evaluate_def, opt_res_rel_def]
       >> imp_res_tac evaluate_SING_IMP
-      >> gvs []
-      >> gvs [hole_unchanged_def, hole_unchanged'_def])
+      >> gvs [holes_unchanged_except_def])
     >> first_x_assum $ qspec_then ‘F’ mp_tac
     >> gvs []
     >> disch_then drule
@@ -1323,81 +1335,8 @@ Proof
     >> Cases_on ‘v'’ >> gvs []
     >> rename [‘state_rel f'' t t'’]
     >> rename [‘v_rel f'' v v'’]
-    >> 
-                                
-
-
-
-       
-    >> gvs []
-    >> strip_tac        
-    >> Cases_on ‘opt’ >> gvs []
-    (* Opt *)
-    (* First inductive hypothesis *)                   
-    >-
-     (first_x_assum $ drule_at Any
-      >> drule env_rel_non_opt
-      >> strip_tac
-      >> gvs []
-      >> rename [‘env_rel F f env env2’]
-      >> Cases_on ‘rs’ >> gvs []
-      >-
-       (rename [‘evaluate (xs,env,s) = (Rval vs,u)’]
-        >> disch_then drule
-        >> strip_tac
-        >> gvs []
-        >> rename [‘evaluate (xs,env2,s') = (Rval vs',u')’]
-        >> drule evaluate_pad_env_val
-        >> strip_tac
-        >> gvs []                        
-        >> Cases_on ‘do_app op (REVERSE vs) u’ >> gvs []
-        >-
-         (Cases_on ‘a’ >> gvs []
-          >> rename [‘do_app op (REVERSE vs) u = Rval (v,t)’]
-          >> drule state_rel_do_app
-          >> disch_then drule
-                        
-          >> drule_all do_app_rewrite_tmc
-          >> strip_tac
-          >> rename [‘f' ⊑ f''’]
-          >> Cases_on ‘r'’ >> gvs []
-          >> Cases_on ‘a’ >> gvs []
-          >> Cases_on ‘a'’ >> gvs []
-          >> rename [‘state_rel f'' t t'’]
-          >> rename [‘v_rel f'' v v'’]
-          >> goal_assum $ drule_at Any
-          >> gvs []
-          >> conj_tac
-          >- imp_res_tac SUBMAP_TRANS
-          >> rw []
-          >- goal_assum $ drule_at Any
-          >> reverse $ Cases_on ‘is_block_op_cons op’ >> gvs[]
-          >-
-           (drule_all aux_strip_op
-            >> strip_tac
-            >> gvs [evaluate_def]
-            (* HERE *)
-                   
-            >> Cases_on ‘i < LENGTH env2 + 2’ >> gvs []
-            >- (Cases_on ‘j < LENGTH env2 + 2’ >> gvs []
-                >-
-                 (CASE_TAC >> gvs []
-                                  
-                                                        
-                  >> Cases_on ‘a’ >> gvs []
-                  >> Cases_on ‘v’ >> Cases_on ‘v'’ >> gvs [v_rel_cases]
-                  >> gvs [do_app_def]
-                         
-                  >> gvs [do_app_def, do_app_aux_def]
-                               
-                  >> gvs [do_app_def]
-                  >> cheat)
-                >> cheat)
-            >> cheat)
-          >> cheat)
-        >> cheat)
-      >> cheat)
-    >> cheat)
+    >> cheat
+   )
   >~ [‘Tick x’] >-
    (gvs [evaluate_def]
     >> ‘s'.clock = s.clock’ by gvs [state_rel_def]
@@ -1409,15 +1348,14 @@ Proof
       >> gvs []
       >> rw []
       >- gvs [only_fresh_refl]
+      >- irule holes_unchanged_except_refl
       >-
        (goal_assum $ drule_at Any
         >> drule aux_strip_tick
         >> strip_tac
         >> gvs [evaluate_def])
-      >-
-        (goal_assum $ drule_at Any
-         >> gvs [rewrite_opt_def, evaluate_def, opt_res_rel_def])
-      >> gvs [hole_unchanged_refl])
+      >> goal_assum $ drule_at Any
+      >> gvs [rewrite_opt_def, evaluate_def, opt_res_rel_def, holes_unchanged_except_refl])
     >> Cases_on ‘opt’ >> gvs []
     (* Opt *)
     >-
